Full printer for Low*

src/arch/x64/interop/Main.ml
@@ -2,4 +2,4 @@ open Interop_Printer
 
 let _ = print_string (translate_vale Linux X86 memcpy)
 let _ = print_newline()
-let _ = print_string (translate_lowstar memcpy)
+let _ = print_string (translate_lowstar Linux X86 memcpy)
