src/arch/x64/interop/Interop_Printer.fst
@@ -90,11 +90,52 @@ let rec disjoint args =
   in aux q ^ disjoint_aux q
   end in disjoint_aux args
 
-let translate_lowstar (func:func_ty) =
+let supported os target args = 
+  List.Tot.Base.length args <= List.Tot.Base.length (calling_registers os target)
+
+let supported_func os target func =
+  let _, args = func in
+  supported os target args
+
+let reg_to_low = function
+  | "rax" -> "Rax"
+  | "rbx" -> "Rbx"
+  | "rcx" -> "Rcx"
+  | "rdx" -> "Rdx"
+  | "rsi" -> "Rsi"
+  | "rdi" -> "Rdi"
+  | "rbp" -> "Rbp"
+  | "rsp" -> "Rsp"
+  | "r8" -> "R8"
+  | "r9" -> "R9"
+  | "r10" -> "R10"
+  | "r11" -> "R11"
+  | "r12" -> "R12"
+  | "r13" -> "R13"
+  | "r14" -> "R14"
+  | "r15" -> "R15"
+  | _ -> "error"
+
+let print_low_calling_args os target (args:list arg{supported os target args}) =
+  let rec aux regs (args:list arg{List.Tot.Base.length args <= List.Tot.Base.length regs}) =
+  match regs, args with
+    | _, [] -> "    | _ -> n"
+    | r1::rn, (a, ty)::q -> "    | " ^ (reg_to_low r1) ^ " -> " ^ 
+      (if TBuffer? ty then "addrs.[(as_addr " ^ a ^ ", idx " ^ a ^ ", length " ^ a ^ ")]" else a) ^ 
+      "\n" ^ aux rn q
+  in aux (calling_registers os target) args
+
+let print_low_callee_saved os target =
+  let rec aux = function
+    | [] -> ""
+    | a::q -> "  assert(s0.regs " ^ (reg_to_low a) ^ " == s1.regs " ^ (reg_to_low a) ^ ");\n" ^ aux q
+  in aux (callee_saved os target)
+
+let translate_lowstar os target (func:func_ty{supported_func os target func}) =
   let name, args = func in
   let separator1 = if (List.Tot.Base.length (List.Tot.Base.filter is_buffer args) <= 1) then "" else " /\\ " in  
   "module " ^ name ^
-  "\n\nopen FStar.Buffer\nmodule B = FStar.Buffer\nopen FStar.HyperStack.ST\nmodule HS = FStar.HyperStack\nopen Interop64\nopen Words_s\nopen Types_s\nmodule S = X64.Bytes_Semantics_s\nopen X64.Machine_s\nopen X64.Memory_i_s\n#set-options \"--z3rlimit 40\"\n\n" ^
+  "\n\nopen FStar.Buffer\nmodule B = FStar.Buffer\nopen FStar.HyperStack.ST\nmodule HS = FStar.HyperStack\nopen Interop64\nopen Words_s\nopen Types_s\nopen X64.Machine_s\nopen X64.Memory_i_s\nopen X64.Vale.State_i\nopen X64.Vale.Decls_i\n#set-options \"--z3rlimit 40\"\n\n" ^
   "assume val st_put (h:HS.mem) (f:HS.mem -> GTot HS.mem) : ST unit (fun h0 -> True) (fun h0 _ h1 -> h == h1 /\ f h0 == h)\n\n" ^
   "// TODO: Complete with your pre- and post-conditions\n" ^
   "let pre_cond (h:HS.mem) " ^ (print_args_list args) ^ "= " ^ (liveness "h" args) ^ separator1 ^ (disjoint args) ^ "\n" ^
@@ -111,16 +152,22 @@ let translate_lowstar (func:func_ty) =
   "#set-options \"--initial_fuel 4 --max_fuel 4 --initial_ifuel 2 --max_ifuel 2\"\n" ^
   "let ghost_" ^ name ^ " " ^ (print_args_names args) ^ "h0 =\n" ^
   "  let buffers = " ^ print_buffers_list args ^ " in\n" ^
-  "  let s0_heap = down_mem64 h0 addrs buffers in\n" ^
   "  let (mem:mem) = {addrs = addrs; ptrs = buffers; hs = h0} in\n" ^
   "  let n:nat64 = 0 in\n" ^    
-  // TODO : Calling conventions for regs
-  "  let regs = fun r -> n in\n" ^
+  "  let regs = fun r -> begin match r with\n" ^
+  (print_low_calling_args os target args) ^
+  " end in\n" ^
   "  let n:nat32 = 0 in\n" ^  
   "  let xmms = fun x -> Mkfour n n n n in\n" ^
-  "  let bytes_s0 = {S.ok = true; S.regs = regs; S.xmms = xmms; S.flags = 0; S.mem = s0_heap} in\n" ^
-  "  let s0 = {state = bytes_s0; mem = mem} in\n" ^
-  "  admit()\n\n" ^
+  "  let s0 = {ok = true; regs = regs; xmms = xmms; flags = 0; mem = mem} in\n" ^
+  "  let s1, f1 = va_lemma_" ^ name ^ " (va_code_" ^ name ^ " ()) s0 " ^ print_args_names args ^ " in\n" ^
+  "  // Ensures that the Vale execution was correct\n" ^
+  "  assert(s1.ok);\n" ^
+  "  // Ensures that the callee_saved registers are correct\n" ^
+  (print_low_callee_saved os target) ^
+  "  // Ensures that va_code_" ^ name ^ " is actually Vale code, and that s1 is the result of executing this code\n" ^
+  "  assert (va_ensure_total (va_code_" ^ name ^ " ()) s0 s1 f1);\n" ^
+  "  s1.mem.hs\n\n" ^
   "let " ^ name ^ " " ^ (print_args_names args) ^ " =\n" ^
   "  let h0 = get() in\n" ^
   "  st_put h0 (fun h -> if FStar.StrongExcludedMiddle.strong_excluded_middle (pre_cond h " ^ (print_args_names args) ^ ") then ghost_" ^ name ^ " " ^ (print_args_names args) ^ "h else h)\n"
@@ -148,13 +195,6 @@ let rec print_vale_loc_buff = function
 let rec print_buff_readable = function
   | [] -> ""
   | (a, _)::q -> "        buffer_readable(mem, "^a^");\n" ^ print_buff_readable q
-
-let supported os target args = 
-  List.Tot.Base.length args <= List.Tot.Base.length (calling_registers os target)
-
-let supported_func os target func =
-  let _, args = func in
-  supported os target args
 
 let print_calling_args os target (args:list arg{supported os target args}) =
   let rec aux regs (args:list arg{List.Tot.Base.length args <= List.Tot.Base.length regs}) =
@@ -196,5 +236,5 @@ let translate_vale os target (func:func_ty{supported_func os target func}) =
 
 let memcpy = ("memcpy", [("src", TBuffer TUInt64); ("dest", TBuffer TUInt64)])
 
-let _ = translate_lowstar memcpy
+let _ = translate_lowstar Linux X86 memcpy
 let _ = translate_vale Linux X86 memcpy
